making extracted wysteria interpreter code to compile in OCaml. had to adjust for projectors and discriminators for indexed types.

examples/wysteria/interpreter_lib.ml
@@ -1,0 +1,29 @@
+module OrdSet = struct
+    type ('a, 'b) ordset = 'a BatSet.t
+
+    let empty _ = BatSet.empty
+    let union _ s1 s2 = BatSet.union s1 s2
+    let intersect _ s1 s2 = BatSet.intersect s1 s2
+    let mem _ x s = BatSet.mem x s					    
+    let choose _ s = BatSet.choose s
+    let remove _ x s = BatSet.remove x s
+    let size _ s = BatSet.cardinal s			       
+    let subset _ s1 s2 = BatSet.subset s1 s2
+    let singleton _ x = BatSet.singleton x
+    let is_singleton _ s = BatSet.cardinal s = 1
+    let insert _ x s = BatSet.add x s
+    let fold _ f s a = BatSet.fold f s a
+end
+
+module OrdMap = struct
+    type ('a, 'b, 'c) ordmap = ('a, 'b) BatMap.t
+
+    let empty _ = BatMap.empty					 
+    let const_on g s x = OrdSet.fold g (fun y m -> BatMap.add y x m) s BatMap.empty
+    let select _ k m = if BatMap.mem k m then Some (BatMap.find k m) else None
+    let update _ k v m = BatMap.add k v m
+    let contains _ k m = BatMap.mem k m
+    let remove _ k m = BatMap.remove k m			    
+    let choose _ m = if not (BatMap.is_empty m) then Some (BatMap.choose m) else None
+    let size _ m = BatMap.cardinal m    				   
+end
